lib_list/Test.LList.fst
@@ -1,0 +1,29 @@
+module Test.LList
+
+
+open Steel.Memory
+open Steel.Effect.Atomic
+open Steel.Effect
+open Steel.Reference
+
+module U64 = FStar.UInt64
+
+open Selectors.LList
+
+let temp (_:unit)
+  : Steel (t U64.t)
+  emp
+  (fun ptr -> llist (fun _ -> emp) ptr)
+  (requires fun _ -> True)
+  (ensures fun _ ptr h1 ->
+    v_llist (fun _ -> emp) ptr h1 == [ 1UL ; 0UL ]
+  )
+  =
+  let c1 = mk_cell null_t 0UL in
+  let r1 = malloc c1 in
+  let c2 = mk_cell r1 1UL in
+  let r2 = malloc c2 in
+  intro_llist_nil U64.t (fun _ -> emp);
+  intro_llist_cons (fun _ -> emp) r1 null_t 0UL;
+  intro_llist_cons (fun _ -> emp) r2 r1 1UL;
+  r2
